DynamoDbEncryption/runtimes/java/src/test/java/software/aws/cryptography/dynamoDbEncryption/OtherTests.java
@@ -15,7 +15,6 @@ import software.amazon.cryptography.dynamoDbEncryption.transforms.model.OpaqueEr
 import software.amazon.cryptography.materialProviders.IBranchKeyIdSupplier;
 import software.amazon.cryptography.materialProviders.IKeyring;
 import software.amazon.cryptography.dynamoDbEncryption.itemEncryptor.model.DynamoDbItemEncryptorConfig;
-import software.amazon.cryptography.materialProviders.IKeyring;
 import software.amazon.cryptography.materialProviders.MaterialProviders;
 import software.amazon.cryptography.materialProviders.model.*;
 import software.amazon.cryptography.structuredEncryption.model.CryptoAction;
