DynamoDbEncryption/dafny/DynamoDbEncryptionTransforms/test/TestFixtures.dfy
@@ -22,6 +22,10 @@ module TestFixtures {
     map["bar" := CSE.SIGN_ONLY, "encrypt" := CSE.ENCRYPT_AND_SIGN, "sign" := CSE.SIGN_ONLY, "nothing" := CSE.DO_NOTHING]
   }
 
+  function method GetSignedAttributeActions() : AttributeActions {
+    map["bar" := CSE.SIGN_ONLY, "encrypt" := CSE.ENCRYPT_AND_SIGN, "sign" := CSE.SIGN_ONLY]
+  }
+
   method GetEncryptorConfig() returns (output : DynamoDbItemEncryptorConfig) {
     var keyring := GetKmsKeyring();
     output := DynamoDbItemEncryptorConfig(
